Fstar/fun/Implmenetations/Utils.Heap.fst
@@ -1,0 +1,60 @@
+module Utils.Heap
+
+// maybe change to generating OCaml maps!
+// OrdMap is an OrdSet: which is just an
+// abstraction over a sorted list!
+module Map = FStar.OrdMap
+module Set = FStar.OrdSet
+
+
+// free is the next free value label
+unopteq type t (a : Type) : Type = {
+  size    : int;
+  free    : l : (list int){Cons? l};
+  maps_to : Map.ordmap int a (<=)
+}
+
+val initial (#a : Type) : (t a)
+let initial #a = {
+  size = 0;
+  free = [1];
+  maps_to = Map.empty
+}
+
+
+val alloc (#a : Type) : t a -> a -> t a * int
+let alloc #a {size; free; maps_to} v =
+  let curr, next_frees =
+    match free with
+    | [x]    -> x, [x + 1]
+    | x :: xs -> x, xs
+  in ({ size    = size + 1;
+        free    = next_frees;
+        maps_to = Map.update curr v maps_to
+      }, curr)
+
+val update (#a : Type) : t a -> int -> a -> t a
+let update #a heap key val' =
+  {heap with maps_to = Map.update key val'  heap.maps_to}
+
+val h_free (#a : Type) : t a -> int -> t a
+let h_free #a {size; free; maps_to} key = {
+  size    = size - 1;
+  free    = key :: free;
+  maps_to = Map.remove key maps_to
+}
+
+// For some reason as_list is private, but we can make it with fold
+private val set_as_list (#a:eqtype) (#acc:Type) (#f:Set.cmp a) : Set.ordset a f -> list a
+private let set_as_list #_ #_ #_ =
+  Set.fold (fun acc x -> x :: acc) []
+
+val addresses (#a : Type) : t a -> list int
+let addresses #a {size; free; maps_to} =
+   set_as_list #int #int (Map.dom maps_to)
+
+val lookup (#a : Type) : t a -> int -> Prims.Tot (option a)
+let lookup #_ {maps_to} val' = Map.select val' maps_to
+
+val size (#a : Type) : t a -> int
+let size #a = Mkt?.size
